pcuic/theories/PCUICSR.v
@@ -26,17 +26,6 @@ Ltac my_rename_hyp h th :=
 
 Ltac rename_hyp h ht ::= my_rename_hyp h ht.
 
-Derive NoConfusion for term.
-
-Lemma mkApps_Fix_eq mfix idx args t : mkApps (tFix mfix idx) args = t ->
-                                      fst (decompose_app t) = (tFix mfix idx).
-Proof.
-  intros H; apply (f_equal decompose_app) in H.
-  rewrite decompose_app_mkApps in H. reflexivity.
-  destruct t; noconf H. rewrite <- H. reflexivity.
-  reflexivity.
-Qed.
-
 Lemma mkApps_Fix_spec mfix idx args t : mkApps (tFix mfix idx) args = t ->
                                       match decompose_app t with
                                       | (tFix mfix idx, args') => args' = args
